theories/prelude/fin_map_dom.v
@@ -1,12 +1,14 @@
 (*
- * Copyright (c) 2022 BedRock Systems, Inc.
+ * Copyright (c) 2022-2024 BedRock Systems, Inc.
  * This software is distributed under the terms of the BedRock Open-Source License.
  * See the LICENSE-BedRock file in the repository root for details.
  *)
 
 Require Import stdpp.fin_map_dom.
 Require Import bedrock.prelude.base.
+Require Import bedrock.prelude.list_numbers.
 Require Import bedrock.prelude.fin_maps.
+Require Import bedrock.prelude.fin_sets.
 Section fin_map_dom.
   Context `{FinMapDom K M D}.
   Context {A : Type}.
@@ -17,3 +19,34 @@ Section fin_map_dom.
     (k, v) ∈ map_to_list m → k ∈ dom m.
   Proof. move=> /elem_of_map_to_list. apply elem_of_dom_2. Qed.
 End fin_map_dom.
+
+Section dom_map_seqZ.
+  Import list_numbers.
+  #[local] Open Scope Z_scope.
+  Context  `{!∀ A, Dom (M A) D, !FMap M,
+               HL : !∀ A, Lookup Z A (M A),
+               HE : !∀ A, Empty (M A),
+               HP : !∀ A, PartialAlter Z A (M A)}.
+  Context `{!Singleton Z D, !Union D, !Intersection D, !Difference D}.
+  Context `{!OMap M, !Merge M, HF : !∀ A, MapFold Z A (M A),
+            !ElemOf Z D, !Empty D, !FinMapDom Z M D}.
+
+  Lemma dom_seqZ {A} (start : Z) (xs : list A) :
+    dom (map_seqZ start xs : M A) ≡ (set_seqZ start (start + lengthZ xs) : D).
+  Proof using FinMapDom0.
+    rewrite /set_seqZ.
+    elim: xs start => [|x xs IH] start.
+    - rewrite lengthN_nil /= Z.add_0_r seqZ_oob //; apply dom_empty.
+    - have ? : (start < start + (lengthN xs + 1)%N) by lia.
+      rewrite [X in dom X] /= dom_insert lengthN_cons seqZ_cons //.
+      rewrite N.add_1_r N2Z.inj_succ -Z.add_succ_comm Z.add_1_r.
+      by rewrite /= -IH.
+  Qed.
+
+  Lemma dom_seqZ_L `{!LeibnizEquiv D, A} (start : Z) (xs : list A) :
+    dom (map_seqZ start xs : M A) = (set_seqZ start (start + lengthN xs) : D).
+  Proof using FinMapDom0.
+    apply leibniz_equiv, dom_seqZ.
+  Qed.
+
+End dom_map_seqZ.
